
\textbf{Column 1: -}

It is the only column that is guaranteed to have no other additional non-zero elements.
\begin{minipage}{0.45\textwidth}
\includegraphics[width=0.45\textwidth]{./Scheduler/PpT-Symbolic_A00.png}
\end{minipage}%
\hfill
\begin{minipage}{0.85\textwidth}
According to equation \ref{eqn:LUD:LUequation0},\\
$U_{1,1}=A_{1,1}$
\end{minipage}

\begin{minipage}{0.45\textwidth}
\includegraphics[width=0.45\textwidth]{./Scheduler/PpT-Symbolic_A01.png}
\end{minipage}%
\hfill
\begin{minipage}{0.85\textwidth}
According to equation \ref{eqn:LUD:LUequation1},\\
$L_{2,1}=0$
\end{minipage}

\begin{minipage}{0.45\textwidth}
\includegraphics[width=0.45\textwidth]{./Scheduler/PpT-Symbolic_A02.png}
\end{minipage}%
\hfill
\begin{minipage}{0.85\textwidth}
According to equation \ref{eqn:LUD:LUequation1},\\
$L_{3,1}=A_{3,1}/U_{1,1}$
\end{minipage}

\begin{minipage}{0.45\textwidth}
\includegraphics[width=0.45\textwidth]{./Scheduler/PpT-Symbolic_A03.png}
\end{minipage}%
\hfill
\begin{minipage}{0.85\textwidth}
According to equation \ref{eqn:LUD:LUequation1},\\
$L_{4,1}=A_{4,1}/U_{1,1}$
\end{minipage}
\\\\
\textbf{Column 2: -}

\begin{minipage}{0.45\textwidth}
\includegraphics[width=0.45\textwidth]{./Scheduler/PpT-Symbolic_A10.png}
\end{minipage}%
\hfill
\begin{minipage}{0.85\textwidth}
According to equation \ref{eqn:LUD:LUequation0},\\
$U_{1,2}=0$
\end{minipage}

\begin{minipage}{0.45\textwidth}
\includegraphics[width=0.45\textwidth]{./Scheduler/PpT-Symbolic_A11.png}
\end{minipage}%
\hfill
\begin{minipage}{0.85\textwidth}
According to equation \ref{eqn:LUD:LUequation0},\\
$U_{2,2}=A_{2,2}$
\end{minipage}

\begin{minipage}{0.45\textwidth}
\includegraphics[width=0.45\textwidth]{./Scheduler/PpT-Symbolic_A12.png}
\end{minipage}%
\hfill
\begin{minipage}{0.85\textwidth}
According to equation \ref{eqn:LUD:LUequation1},\\
$L_{3,2}=0$
\end{minipage}

\begin{minipage}{0.45\textwidth}
\includegraphics[width=0.45\textwidth]{./Scheduler/PpT-Symbolic_A13.png}
\end{minipage}%
\hfill
\begin{minipage}{0.85\textwidth}
According to equation \ref{eqn:LUD:LUequation1},\\
$L_{4,2}=A_{4,2}/U_{2,2}$
\end{minipage}
\\\\
\textbf{Column 3: -}

\begin{minipage}{0.45\textwidth}
\includegraphics[width=0.45\textwidth]{./Scheduler/PpT-Symbolic_A20.png}
\end{minipage}%
\hfill
\begin{minipage}{0.85\textwidth}
According to equation \ref{eqn:LUD:LUequation0},\\
$U_{1,3}=A_{1,3}$
\end{minipage}

\begin{minipage}{0.45\textwidth}
\includegraphics[width=0.45\textwidth]{./Scheduler/PpT-Symbolic_A21.png}
\end{minipage}%
\hfill
\begin{minipage}{0.85\textwidth}
According to equation \ref{eqn:LUD:LUequation0},\\
$U_{2,3}=0$
\end{minipage}


\begin{minipage}{0.45\textwidth}
\includegraphics[width=0.45\textwidth]{./Scheduler/PpT-Symbolic_A22.png}
\end{minipage}%
\hfill
\begin{minipage}{0.85\textwidth}
According to equation \ref{eqn:LUD:LUequation0},\\
$U_{3,3}=-(L_{3,1} \cdot U_{1,2})$
\end{minipage}

\begin{minipage}{0.45\textwidth}
\includegraphics[width=0.45\textwidth]{./Scheduler/PpT-Symbolic_A23.png}
\end{minipage}%
\hfill
\begin{minipage}{0.85\textwidth}
According to equation \ref{eqn:LUD:LUequation1},\\
$ L_{4,3}=A_{4,3} - ( L_{4,1} \cdot U_{1.3} )/U_{3,3} $
\end{minipage}
\\\\
\textbf{Column 4: -}

\begin{minipage}{0.45\textwidth}
\includegraphics[width=0.45\textwidth]{./Scheduler/PpT-Symbolic_A30.png}
\end{minipage}%
\hfill
\begin{minipage}{0.85\textwidth}
According to equation \ref{eqn:LUD:LUequation0},\\
$U_{1,4}=0$
\end{minipage}

\begin{minipage}{0.45\textwidth}
\includegraphics[width=0.45\textwidth]{./Scheduler/PpT-Symbolic_A31.png}
\end{minipage}%
\hfill
\begin{minipage}{0.85\textwidth}
According to equation \ref{eqn:LUD:LUequation0},\\
$U_{2,4}=A_{2,4}$
\end{minipage}

\begin{minipage}{0.45\textwidth}
\includegraphics[width=0.45\textwidth]{./Scheduler/PpT-Symbolic_A32.png}
\end{minipage}%
\hfill
\begin{minipage}{0.85\textwidth}
According to equation \ref{eqn:LUD:LUequation0},\\
$U_{3,4}=A_{3,4}$
\end{minipage}

\begin{minipage}{0.45\textwidth}
\includegraphics[width=0.45\textwidth]{./Scheduler/PpT-Symbolic_A33.png}
\end{minipage}%
\hfill
\begin{minipage}{0.85\textwidth}
According to equation \ref{eqn:LUD:LUequation0},\\
$U_{4,4}= - (L_{4,2}\cdot U_{2,4} )$
\end{minipage}